Logic/Modal/Standard/PLoN/Semantics.lean
@@ -50,67 +50,67 @@ variable {α : Type*}
 
 open Standard.PLoN
 
-def Formula.plon_satisfies (M : PLoN.Model α) (w : M.World) : Formula α → Prop
+def Formula.PLoN.Satisfies (M : PLoN.Model α) (w : M.World) : Formula α → Prop
   | atom a  => M.Valuation w a
   | verum   => True
   | falsum  => False
-  | and p q => (p.plon_satisfies M w) ∧ (q.plon_satisfies M w)
-  | or p q  => (p.plon_satisfies M w) ∨ (q.plon_satisfies M w)
-  | imp p q => (p.plon_satisfies M w) → (q.plon_satisfies M w)
-  | box p   => ∀ {w'}, w ≺[p] w' → (p.plon_satisfies M w')
+  | and p q => (PLoN.Satisfies M w p) ∧ (PLoN.Satisfies M w q)
+  | or p q  => (PLoN.Satisfies M w p) ∨ (PLoN.Satisfies M w q)
+  | imp p q => (PLoN.Satisfies M w p) → (PLoN.Satisfies M w q)
+  | box p   => ∀ {w'}, w ≺[p] w' → (PLoN.Satisfies M w' p)
 
 
-namespace Formula.plon_satisfies
+namespace Formula.PLoN.Satisfies
 
-protected instance semantics (M : PLoN.Model α) : Semantics (Formula α) (M.World) := ⟨fun w ↦ Formula.plon_satisfies M w⟩
+protected instance semantics (M : PLoN.Model α) : Semantics (Formula α) (M.World) := ⟨fun w ↦ Formula.PLoN.Satisfies M w⟩
 
 variable {M : PLoN.Model α} {w : M.World} {p q : Formula α}
 
-@[simp] protected lemma iff_models : w ⊧ p ↔ p.plon_satisfies M w := by rfl
+@[simp] protected lemma iff_models : w ⊧ p ↔ PLoN.Satisfies M w p := by rfl
 
 instance : Semantics.Tarski M.World where
-  realize_top := by simp [plon_satisfies];
-  realize_bot := by simp [plon_satisfies];
-  realize_not := by simp [plon_satisfies];
-  realize_and := by simp [plon_satisfies];
-  realize_or  := by simp [plon_satisfies];
-  realize_imp := by simp [plon_satisfies];
+  realize_top := by simp [PLoN.Satisfies];
+  realize_bot := by simp [PLoN.Satisfies];
+  realize_not := by simp [PLoN.Satisfies];
+  realize_and := by simp [PLoN.Satisfies];
+  realize_or  := by simp [PLoN.Satisfies];
+  realize_imp := by simp [PLoN.Satisfies];
 
-end Formula.plon_satisfies
+end Formula.PLoN.Satisfies
 
 
-def Formula.valid_on_PLoNModel (M : PLoN.Model α) (p : Formula α) : Prop := ∀ w : M.World, w ⊧ p
+def Formula.PLoN.ValidOnModel (M : PLoN.Model α) (p : Formula α) : Prop := ∀ w : M.World, w ⊧ p
 
-namespace Formula.valid_on_PLoNModel
+namespace Formula.PLoN.ValidOnModel
 
-instance : Semantics (Formula α) (PLoN.Model α) := ⟨fun M ↦ Formula.valid_on_PLoNModel M⟩
+instance : Semantics (Formula α) (PLoN.Model α) := ⟨fun M ↦ Formula.PLoN.ValidOnModel M⟩
 
 @[simp]
 protected lemma iff_models {M : PLoN.Model α} {p : Formula α}
-: M ⊧ p ↔ Formula.valid_on_PLoNModel M p := by rfl
+: M ⊧ p ↔ Formula.PLoN.ValidOnModel M p := by rfl
 
 instance : Semantics.Bot (PLoN.Model α) where
   realize_bot _ := by
-    simp [Formula.valid_on_PLoNModel];
+    simp [Formula.PLoN.ValidOnModel];
     use ﹫;
 
-end Formula.valid_on_PLoNModel
+end Formula.PLoN.ValidOnModel
 
 
-def Formula.valid_on_PLoNFrame (F : PLoN.Frame α) (p : Formula α) := ∀ V, (Model.mk F V) ⊧ p
+def Formula.PLoN.ValidOnFrame (F : PLoN.Frame α) (p : Formula α) := ∀ V, (Model.mk F V) ⊧ p
 
-namespace Formula.valid_on_PLoNFrame
+namespace Formula.PLoN.ValidOnFrame
 
-instance : Semantics (Formula α) (PLoN.Frame α) := ⟨fun F ↦ Formula.valid_on_PLoNFrame F⟩
+instance : Semantics (Formula α) (PLoN.Frame α) := ⟨fun F ↦ Formula.PLoN.ValidOnFrame F⟩
 
 @[simp]
 protected lemma iff_models {F : PLoN.Frame α} {p : Formula α}
-: F ⊧ p ↔ Formula.valid_on_PLoNFrame F p := by rfl
+: F ⊧ p ↔ Formula.PLoN.ValidOnFrame F p := by rfl
 
 variable {F : Frame α}
 
 instance : Semantics.Bot (PLoN.Frame α) where
-  realize_bot _ := by simp [Formula.valid_on_PLoNFrame];
+  realize_bot _ := by simp [Formula.PLoN.ValidOnFrame];
 
 protected lemma nec (h : F ⊧ p) : F ⊧ □p := by
   intro V x y _;
@@ -120,30 +120,30 @@ protected lemma mdp (hpq : F ⊧ p ⟶ q) (hp : F ⊧ p) : F ⊧ q := by
   intro V x;
   exact (hpq V x) (hp V x);
 
-end Formula.valid_on_PLoNFrame
+end Formula.PLoN.ValidOnFrame
 
 
-def Formula.valid_on_PLoNFrameClass (𝔽 : PLoN.FrameClass α) (p : Formula α) := ∀ {F}, F ∈ 𝔽 → F ⊧ p
+def Formula.PLoN.ValidOnFrameClass (𝔽 : PLoN.FrameClass α) (p : Formula α) := ∀ {F}, F ∈ 𝔽 → F ⊧ p
 
-namespace Formula.valid_on_PLoNFrameClass
+namespace Formula.PLoN.ValidOnFrameClass
 
-instance : Semantics (Formula α) (PLoN.FrameClass α) := ⟨fun 𝔽 ↦ Formula.valid_on_PLoNFrameClass 𝔽⟩
+instance : Semantics (Formula α) (PLoN.FrameClass α) := ⟨fun 𝔽 ↦ Formula.PLoN.ValidOnFrameClass 𝔽⟩
 
 variable {𝔽 : FrameClass α}
 
 @[simp]
-protected lemma iff_models {𝔽 : PLoN.FrameClass α} {p : Formula α} : 𝔽 ⊧ p ↔ Formula.valid_on_PLoNFrameClass 𝔽 p := by rfl
+protected lemma iff_models {𝔽 : PLoN.FrameClass α} {p : Formula α} : 𝔽 ⊧ p ↔ Formula.PLoN.ValidOnFrameClass 𝔽 p := by rfl
 
 protected lemma nec (h : 𝔽 ⊧ p) : 𝔽 ⊧ □p := by
   intro _ hF;
-  apply valid_on_PLoNFrame.nec;
+  apply PLoN.ValidOnFrame.nec;
   exact h hF;
 
 protected lemma mdp (hpq : 𝔽 ⊧ p ⟶ q) (hp : 𝔽 ⊧ p) : 𝔽 ⊧ q := by
   intro _ hF;
-  exact valid_on_PLoNFrame.mdp (hpq hF) (hp hF)
+  exact PLoN.ValidOnFrame.mdp (hpq hF) (hp hF)
 
-end Formula.valid_on_PLoNFrameClass
+end Formula.PLoN.ValidOnFrameClass
 
 
 def DeductionParameter.DefinesPLoNFrameClass (𝓓 : DeductionParameter α) (𝔽 : PLoN.FrameClass α) := ∀ {F : Frame α}, F ⊧* 𝓓.theory ↔ F ∈ 𝔽
@@ -161,7 +161,7 @@ open Formula
 
 lemma N_defines : 𝐍.DefinesPLoNFrameClass (AllFrameClass α) := by
   intro F;
-  simp [DeductionParameter.theory, System.theory, valid_on_PLoNFrame, valid_on_PLoNModel];
+  simp [DeductionParameter.theory, System.theory, PLoN.ValidOnFrame, PLoN.ValidOnModel];
   intro p hp;
   induction hp using Deduction.inducition_with_necOnly! with
   | hMaxm h => simp at h;
@@ -172,12 +172,12 @@ lemma N_defines : 𝐍.DefinesPLoNFrameClass (AllFrameClass α) := by
     intro V w w' _;
     exact ihp V w';
   | hDisj₃ =>
-    simp_all only [plon_satisfies];
+    simp_all only [PLoN.Satisfies];
     intros; rename_i hpr hqr hpq;
     cases hpq with
     | inl hp => exact hpr hp;
     | inr hq => exact hqr hq;
-  | _ => simp_all [plon_satisfies];
+  | _ => simp_all [PLoN.Satisfies];
 
 end PLoN
 
