Logic/Modal/Standard/Kripke/GL.lean
@@ -18,43 +18,43 @@ private lemma trans_of_L : F# ⊧* (𝗟 : AxiomSet α) → Transitive F.Rel := 
   contrapose;
   intro hT; simp [Transitive] at hT;
   obtain ⟨w₁, w₂, r₁₂, w₃, r₂₃, nr₁₃⟩ := hT;
-  simp [valid_on_KripkeFrame, valid_on_KripkeFrame, valid_on_KripkeModel, kripke_satisfies];
+  simp [Kripke.ValidOnFrame, Kripke.ValidOnFrame, Kripke.ValidOnModel, Kripke.Satisfies];
   use (atom default), (λ w' _ => w' ≠ w₂ ∧ w' ≠ w₃), w₁;
   constructor;
   . intro x hx h;
     by_cases hx₂ : x = w₂;
-    . subst hx₂; simpa [kripke_satisfies] using h r₂₃;
-    . by_cases hx₃ : x = w₃ <;> simp_all [kripke_satisfies, hx₃];
-  . existsi w₂; simpa [kripke_satisfies];
+    . subst hx₂; simpa [Kripke.Satisfies] using h r₂₃;
+    . by_cases hx₃ : x = w₃ <;> simp_all [Kripke.Satisfies, hx₃];
+  . existsi w₂; simpa [Kripke.Satisfies];
 
 private lemma cwf_of_L  : F# ⊧* (𝗟 : AxiomSet α) → ConverseWellFounded F.Rel := by
   contrapose;
   intro hCF;
   obtain ⟨X, hX₁, hX₂⟩ := by simpa using ConverseWellFounded.iff_has_max.not.mp hCF;
-  simp [valid_on_KripkeFrame, valid_on_KripkeFrame, valid_on_KripkeModel, kripke_satisfies];
+  simp [Kripke.ValidOnFrame, Kripke.ValidOnFrame, Kripke.ValidOnModel, Kripke.Satisfies];
   use (atom default), (λ w _ => w ∉ X), hX₁.some;
   constructor;
   . intro x _;
     by_cases hxs : x ∈ X
     . obtain ⟨y, hy₁, hy₂⟩ := hX₂ x hxs;
       intro h;
-      exact h (by simp_all only [kripke_satisfies]);
+      exact h (by simp_all only [Kripke.Satisfies]);
     . aesop;
   . obtain ⟨w', hw'₁, hw'₂⟩ := hX₂ hX₁.some (by apply Set.Nonempty.some_mem);
     existsi w';
     constructor;
     . simpa using hw'₂;
-    . simpa [kripke_satisfies];
+    . simpa [Kripke.Satisfies];
 
 private lemma L_of_trans_and_cwf : (Transitive F.Rel ∧ ConverseWellFounded F.Rel) → F# ⊧* (𝗟 : AxiomSet α) := by
   rintro ⟨hTrans, hWF⟩;
   simp [AxiomSet.L, Axioms.L];
   intro p V w;
-  simp [kripke_satisfies];
+  simp [Kripke.Satisfies];
   contrapose; push_neg;
   intro h;
   obtain ⟨z, rwz, hz⟩ := h;
-  obtain ⟨m, ⟨⟨rwm, hm⟩, hm₂⟩⟩ := hWF.has_min ({ x | (F.Rel w x) ∧ ¬(kripke_satisfies ⟨F, V⟩ x p) }) (by use z; simp_all)
+  obtain ⟨m, ⟨⟨rwm, hm⟩, hm₂⟩⟩ := hWF.has_min ({ x | (F.Rel w x) ∧ ¬(Kripke.Satisfies ⟨F, V⟩ x p) }) (by use z; simp_all)
   use m;
   constructor;
   . exact rwm;
